tests/Delay.v
@@ -24,9 +24,14 @@ Export MonadNotation.
 
 Require Import Cava.Cava.
 Require Import Cava.Monad.CavaMonad.
+Require Import Cava.Lib.UnsignedAdders.
 
 From Coq Require Vector.
 From Coq Require Import Bool.Bvector.
+
+(******************************************************************************)
+(* A byte unit delay.                                                         *)
+(******************************************************************************)
 
 Section WithCava.
   Context {signal} `{Cava signal} `{Monad cava}.
@@ -38,8 +43,12 @@ Section WithCava.
 End WithCava.
 
 Definition b0 := N2Bv_sized 8 0.
-Definition b14 := N2Bv_sized 8 14.
+Definition b3 := N2Bv_sized 8 3.
 Definition b7 := N2Bv_sized 8 7.
+Definition b14 := N2Bv_sized 8 14.
+Definition b18 := N2Bv_sized 8 18.
+Definition b21 := N2Bv_sized 8 21.
+Definition b24 := N2Bv_sized 8 24.
 Definition b250 := N2Bv_sized 8 250.
 
 Local Open Scope list_scope.
@@ -62,6 +71,104 @@ Definition delayByte_Interface
 
 Definition delayByte_Netlist := makeNetlist delayByte_Interface delayByte.
 
+Definition delayByte_tb_inputs := [b14; b7; b250].
+
+Definition delayByte_tb_expected_outputs
+  := sequential (delayByte delayByte_tb_inputs).
+
 Definition delayByte_tb
   := testBench "delayByte_tb" delayByte_Interface
-      [b14; b7; b250]  [b0; b14; b7].
+      delayByte_tb_inputs delayByte_tb_expected_outputs.
+
+(******************************************************************************)
+(* A pipelined NAND gate.                                                     *)
+(******************************************************************************)
+
+Section WithCava.
+  Context {signal} `{Cava signal} `{Monad cava}.
+
+ (* A nand-gate with registers after the AND gate and the INV gate. *)
+  Definition pipelinedNAND : signal Bit * signal Bit -> cava (signal Bit) :=
+    nand2 >=> delay >=> inv >=> delay.
+
+End WithCava.
+
+Definition pipelinedNANDInterface
+  := sequentialInterface "pipelinedNAND"
+     "clk" PositiveEdge "rst" PositiveEdge
+     [mkPort "a" Bit; mkPort "b" Bit]
+     [mkPort "c"  Bit]
+     [].
+
+Definition pipelinedNANDNetlist :=
+  makeNetlist pipelinedNANDInterface pipelinedNAND.
+
+
+Definition pipelinedNAND_tb_inputs
+  := ([true; false;  true; false; true;  false; true; false],
+      [false; false; true; true;  false; false; true; true]
+     ).
+
+Definition pipelinedNAND_tb_expected_outputs
+  := sequential (pipelinedNAND pipelinedNAND_tb_inputs).
+
+Compute list (tupleSimInterface (circuitInputs pipelinedNANDInterface)).
+
+(* TODO(satnam6502): Sequential interface for test-bench generation.
+Definition pipelinedNAND_tb
+  := testBench "pipelinedNAND_tb" pipelinedNANDInterface
+     pipelinedNAND_tb_inputs pipelinedNAND_tb_expected_outputs.
+*)
+
+(******************************************************************************)
+(* countBy                                                                    *)
+(******************************************************************************) 
+
+(*
+
+The countBy circuit takes the current 8-bit input (in) and the current
+state value represented by the register (delay) which is output in the
+current cycle as the output of the circuit, and this value is also the
+next state value for the delay. The adder is an 8-bit adder with no
+bit-growth i.e. it computes (a + b) mod 256.
+
+        _______
+    ---| delay |------------
+   |   |_______|            |
+   |   ___                  |
+    --| + ---------------------- out
+ in --|___|     
+
+*)
+
+Section WithCava.
+  Context {signal} `{Cava signal} `{Monad cava}.
+
+  Definition countFork (i : signal (Vec Bit 8) * signal (Vec Bit 8))
+                       : cava (signal (Vec Bit 8) * signal (Vec Bit 8)) :=
+    newCount <- addN (fst i) (snd i) ;;
+    ret (newCount, newCount).
+
+  Definition countBy : signal (Vec Bit 8) -> cava (signal (Vec Bit 8))
+    := loop countFork.
+
+End WithCava.
+
+Example countBy_ex1: sequential (countBy [b14; b7; b3; b250]) = [b14; b21; b24; b18].
+Proof. reflexivity. Qed.
+
+Local Open Scope N_scope.
+
+Fixpoint countBySpec' (state: N) (i : list (Bvector 8)) 
+                      : list (Bvector 8) :=
+  match i with
+  | [] => []
+  | x::xs => let newState := (Bv2N x + state) mod 256 in
+             N2Bv_sized 8 newState :: countBySpec' newState xs 
+  end.
+
+Definition countBySpec := countBySpec' 0.
+
+Lemma countByCorrect: forall (i : list (Bvector 8)),
+                      sequential (countBy i) = countBySpec i.
+Abort.                      
